Revert ValueInt.v

src/hls/ValueInt.v
@@ -34,10 +34,7 @@ on the size of the [value]. This is necessary so that we can easily store
 
 Using the default [word], this would not be possible, as the size is part of the type. *)
 
-Inductive value : Type :=
-| value_bool : bool -> value
-| value_int : int -> value
-| value_long : int64 -> value.
+Definition value : Type := int.
 
 (** ** Value conversions
 
@@ -45,93 +42,44 @@ Various conversions to different number types such as [N], [Z], [positive] and
 [int], where the last one is a theory of integers of powers of 2 in CompCert. *)
 
 Definition valueToNat (v : value) : nat :=
-  match v with
-  | value_bool b => Nat.b2n b
-  | value_int i => Z.to_nat (Int.unsigned i)
-  | value_long i => Z.to_nat (Int64.unsigned i)
-  end.
+  Z.to_nat (Int.unsigned v).
 
 Definition natToValue (n : nat) : value :=
-  value_int (Int.repr (Z.of_nat n)).
-
-Definition natToValue64 (n : nat) : value :=
-  value_long (Int64.repr (Z.of_nat n)).
+  Int.repr (Z.of_nat n).
 
 Definition valueToN (v : value) : N :=
-  match v with
-  | value_bool b => N.b2n b
-  | value_int i => Z.to_N (Int.unsigned i)
-  | value_long i => Z.to_N (Int64.unsigned i)
-  end.
+  Z.to_N (Int.unsigned v).
 
 Definition NToValue (n : N) : value :=
-  value_int (Int.repr (Z.of_N n)).
-
-Definition NToValue64 (n : N) : value :=
-  value_long (Int64.repr (Z.of_N n)).
+  Int.repr (Z.of_N n).
 
 Definition ZToValue (z : Z) : value :=
-  value_int (Int.repr z).
-Hint Unfold ZToValue : core.
-
-Definition ZToValue64 (z : Z) : value :=
-  value_long (Int64.repr z).
-Hint Unfold ZToValue64 : core.
+  Int.repr z.
 
 Definition valueToZ (v : value) : Z :=
-  match v with
-  | value_bool b => Z.b2z b
-  | value_int i => Int.signed i
-  | value_long i => Int64.signed i
-  end.
-Hint Unfold valueToZ : core.
+  Int.signed v.
 
 Definition uvalueToZ (v : value) : Z :=
-  match v with
-  | value_bool b => Z.b2z b
-  | value_int i => Int.unsigned i
-  | value_long i => Int64.unsigned i
-  end.
-Hint Unfold valueToZ : core.
+  Int.unsigned v.
 
 Definition posToValue (p : positive) : value :=
-  value_int (Int.repr (Z.pos p)).
-
-Definition posToValue64 (p : positive) : value :=
-  value_long (Int64.repr (Z.pos p)).
+  Int.repr (Z.pos p).
 
 Definition valueToPos (v : value) : positive :=
-  match v with
-  | value_bool b => 1%positive
-  | value_int i => Z.to_pos (Int.unsigned i)
-  | value_long i => Z.to_pos (Int64.unsigned i)
-  end.
+  Z.to_pos (Int.unsigned v).
 
-Definition intToValue (i : Integers.int) : value := value_int i.
+Definition intToValue (i : Integers.int) : value := i.
 
-Definition longToValue (i : Integers.int64) : value := value_long i.
+Definition valueToInt (i : value) : Integers.int := i.
 
-Definition valueToInt (v : value) : Integers.int :=
-  match v with
-  | value_bool b => Int.repr (if b then 1 else 0)
-  | value_int i => i
-  | value_long i => Int.repr (Int64.unsigned i)
-  end.
+Definition ptrToValue (i : ptrofs) : value := Ptrofs.to_int i.
 
-Definition ptrToValue (i : ptrofs) : value :=
-  value_int (Ptrofs.to_int i).
-
-Definition valueToPtr (i : value) : ptrofs :=
-  match i with
-  | value_bool b => Ptrofs.repr (if b then 1 else 0)
-  | value_int i => Ptrofs.repr (Int.unsigned i)
-  | value_long i => Ptrofs.repr (Int64.unsigned i)
-  end.
+Definition valueToPtr (i : value) : Integers.ptrofs :=
+  Ptrofs.of_int i.
 
 Definition valToValue (v : Values.val) : option value :=
   match v with
   | Values.Vint i => Some (intToValue i)
-  | Values.Vlong i => Some (longToValue i)
   | Values.Vptr b off => Some (ptrToValue off)
   | Values.Vundef => Some (ZToValue 0%Z)
   | _ => None
@@ -160,11 +108,9 @@ Proof. auto. Qed.
 
 Inductive val_value_lessdef: val -> value -> Prop :=
 | val_value_lessdef_int:
-    forall i,
-    val_value_lessdef (Vint i) (value_int i)
-| val_value_lessdef_long:
-    forall i,
-    val_value_lessdef (Vlong i) (value_long i)
+    forall i v',
+    i = valueToInt v' ->
+    val_value_lessdef (Vint i) v'
 | val_value_lessdef_ptr:
     forall b off v',
     off = valueToPtr v' ->
@@ -180,15 +126,13 @@ Lemma valueToZ_ZToValue :
   forall z,
   (Int.min_signed <= z <= Int.max_signed)%Z ->
   valueToZ (ZToValue z) = z.
-Proof.
-  simpl; auto using Int.signed_repr.
-Qed.
+Proof. auto using Int.signed_repr. Qed.
 
 Lemma uvalueToZ_ZToValue :
   forall z,
   (0 <= z <= Int.max_unsigned)%Z ->
   uvalueToZ (ZToValue z) = z.
-Proof. simpl; auto using Int.unsigned_repr. Qed.
+Proof. auto using Int.unsigned_repr. Qed.
 
 Lemma valueToPos_posToValue :
   forall v,
@@ -211,9 +155,9 @@ Lemma valToValue_lessdef :
     val_value_lessdef v v'.
 Proof.
   intros.
-  destruct v; destruct v'; try discriminate; try constructor.
-  unfold valToValue in H. inversion H. constructor.
-  unfold valToValue, longToValue in *. inv H. constructor.
+  destruct v; try discriminate; constructor.
+  unfold valToValue in H. inversion H.
+  unfold valueToInt. unfold intToValue in H1. auto.
   inv H. symmetry. unfold valueToPtr, ptrToValue. apply Ptrofs.of_int_to_int. trivial.
 Qed.
 
